Lots more module stuff.

module.v
@@ -1,6 +1,7 @@
 Require Import
    Morphisms RelationClasses Equivalence Setoid
    abstract_algebra setoid.
+Require Import rings.
 
 (* me *)
 
@@ -15,7 +16,7 @@ Class Rmodule `(ez: Equiv Scalar) `(ee: Equiv Elem) `{op: RalgebraAction Scalar 
     elem_plus elem_zero elem_opp: Prop :=
   { rmodule_ring: @Ring Scalar ez szalar_plus szalar_mult szalar_zero szalar_one szalar_inv
   ; rmodule_abgroup:> @AbGroup _ _ elem_plus elem_zero elem_opp
-  ; rmodule_action: `(1 <*> x = x)
+  ; rmodule_unital: `(1 <*> x = x)
   ; rmodule_action_proper:> Proper (ez ==> ee ==> ee) op
   ; rmodule_distr_l: `(x <*> (a & b) = (x <*> a) & (x <*> b))
   ; rmodule_distr_r: `((x + y) <*> a = (x <*> a) & (y <*> a))
@@ -30,6 +31,23 @@ Class Ralgebra `(ez: Equiv Scalar) `(e': Equiv Elem) `{RalgebraAction Scalar Ele
   ; ralgebra_ring:> @Ring Elem e' elem_plus elem_mult elem_zero elem_one elem_opp
   ; ralgebra_assoc: `(x <*> (a * b) = (x <*> a) * b) }.
 
+Section Morphisms.
+Context `{Ring R} `{Rmodule R M} {r: R}.
+Global Instance: Setoid_Morphism (ralgebra_action r).
+Global Instance: SemiGroup_Morphism (ralgebra_action r).
+Proof.
+  intuition; constructor; try typeclasses eauto.
+  apply rmodule_distr_l.
+Qed.
+Global Instance: Monoid_Morphism (ralgebra_action r).
+Proof.
+  intuition constructor; try typeclasses eauto.
+  apply (right_cancel (r<*>-mon_unit)).
+  rewrite left_identity.
+  rewrite <- rmodule_distr_l.
+  rewrite left_identity.
+  apply rmodule_action_proper; try reflexivity. 
+Qed.
 
 Global Instance SemiGroup_Morphism_id M `{SemiGroup M}: SemiGroup_Morphism (id: M→M).
 Proof.
@@ -58,26 +76,31 @@ Proof.
   unfold compose; do 2 rewrite preserves_mon_unit; reflexivity.
 Qed.
 
+End Morphisms.
+
 Require Import theory.rings.
 Section Basic_Lemmas.
 Context `{Ring R} `{Rmodule R M}.
-Goal `((-(1)) <*> m = - m).
-  intro m.
+Lemma rmodule_zero_action r: (0 <*> r = mon_unit).
+Proof.
+  apply (left_cancel (1<*>r)).
+  rewrite <- rmodule_distr_r.
+  rewrite (right_identity (1<*>r)).
+  apply rmodule_action_proper; try reflexivity.
+  apply right_identity.
+Qed.
+Lemma rmodule_minus: `((-r) <*> m = -r <*> m).
+Proof.
+  intros r m.
   apply inv_unique; left.
-  setoid_rewrite <- (rmodule_action m) at 1.
   rewrite <- (rmodule_distr_r).
   rewrite plus_opp_r.
-Goal `(0 <*> r = mon_unit).
-Proof.
-  intro m.
-  rewrite <- (left_absorb 0).
-
-Goal `(r <*> mon_unit = mon_unit).
+  apply rmodule_zero_action.
+Qed.
+End Basic_Lemmas.
 
 
-  Typeclasses eauto := .
 Section Rmodules.
-
 
 Class Rmodule_Morphism Scalar M1 M2 {ez: Equiv Scalar} {e1: Equiv M1} `{RalgebraAction Scalar M1} {e2: Equiv M2} `{RalgebraAction Scalar M2}
     {szalar_plus} {szalar_mult} {szalar_zero: RingZero Scalar} {szalar_one: RingOne Scalar} {szalar_inv: GroupInv Scalar}
@@ -85,7 +108,7 @@ Class Rmodule_Morphism Scalar M1 M2 {ez: Equiv Scalar} {e1: Equiv M1} `{Ralgebra
 { rmodule_morphism_ring : @Ring Scalar ez szalar_plus szalar_mult szalar_zero szalar_one szalar_inv
 ; rmodule_morphism_M1_abgroup: @Rmodule Scalar _ M1 _ _ _ _ _ _ _ M1_plus M1_zero M1_opp
 ; rmodule_morphism_M2_abgroup: @Rmodule  Scalar _ M2 _ _ _ _ _ _ _ M2_plus M2_zero M2_opp
-; rmodule_morphism_groupmor:> Group_Morphism f
+; rmodule_morphism_groupmor:> Monoid_Morphism f
 ; preserves_rmodule_action: `(f (x <*> a) = x <*> f a)
 }.
 
@@ -97,18 +120,16 @@ Qed.
 Local Implicit Arguments Rmodule [[ez] [ee] [op]].
 
 Global Instance Rmodule_Morphism_comp (R S T U: Type) `{Ring R}
-  `{Rmodule R S }
- `{ Rmodule R T, Rmodule R U} 
-
- {f: T->U} (g: S->T)
+  `{Rmodule R S, Rmodule R T, Rmodule R U} 
+  {f: T->U} (g: S->T)
   `{!Rmodule_Morphism f} `{!Rmodule_Morphism g}
- : Rmodule_Morphism (compose f g).
-constructor; try typeclasses eauto.
-intros x a.
-unfold compose.
-do 2 rewrite preserves_rmodule_action; reflexivity.
+  : Rmodule_Morphism (compose f g).
+Proof.
+  constructor; try typeclasses eauto.
+  intros x a.
+  unfold compose.
+  do 2 rewrite preserves_rmodule_action; reflexivity.
 Qed.
-
 
 Context `{Ring R}.
 Local Implicit Arguments Rmodule [[ez] [ee] [op] [szalar_plus] [szalar_mult] [szalar_inv] [szalar_zero] [szalar_one]].
@@ -135,7 +156,6 @@ Global Existing Instance arrow_rmodmor.
 Hint Extern 4 (Arrows Object) => exact Arrow: typeclass_instances.
 Section e. Context {M N: Object}.
 Global Instance ea: Equiv (M ⟶ N) := fun f g => ∀ (m: M), f m = g m.
-Typeclasses eauto := debug 10.
 Instance: Equivalence ea.
 Proof. prove_equivalence. Qed.
 
@@ -151,12 +171,13 @@ Global Instance: CatComp Object := fun x y z f g =>  arrow (f:= compose f g) _.
 Global Instance: ∀ x y z: Object,
     Proper (equiv ==> equiv ==> equiv) ((◎): (y ⟶ z) -> (x ⟶ y) -> (x ⟶ z)).
 Proof.
-intros. intros a b Hab c d Hcd.
-unfold equiv, ea.
-simpl.
-unfold compose. unfold equiv, ea in Hab, Hcd. setoid_rewrite  Hab.
-setoid_rewrite Hcd.
-reflexivity.
+  intros. intros a b Hab c d Hcd.
+  unfold equiv, ea.
+  simpl.
+  unfold compose. unfold equiv, ea in Hab, Hcd.
+  setoid_rewrite  Hab.
+  setoid_rewrite Hcd.
+  reflexivity.
 Qed.
 
 Let id_l' (x y: Object) (f: x⟶y): cat_id ◎ f = f.
@@ -164,44 +185,117 @@ Proof. intro; reflexivity. Qed.
 Let id_r' (x y: Object) (f: x⟶y): f ◎ cat_id = f.
 Proof. intro; reflexivity. Qed.
 
-  Lemma comp_assoc' (w x y z: Object) (a: w ⟶ x) (b: x ⟶ y) (c: y ⟶ z): c ◎ (b ◎ a) = (c ◎ b) ◎ a.
-  Proof. intro; reflexivity. Qed.
+Lemma comp_assoc' (w x y z: Object) (a: w ⟶ x) (b: x ⟶ y) (c: y ⟶ z): c ◎ (b ◎ a) = (c ◎ b) ◎ a.
+Proof. intro; reflexivity. Qed.
 
+Global Instance: Category Object := { comp_assoc := comp_assoc'; id_l := id_l'; id_r := id_r'}.
 
-  Global Instance: Category Object := { comp_assoc := comp_assoc'; id_l := id_l'; id_r := id_r'}.
+Section Kernel.
+Context {M N: Type}.
 
-Context M N `{Rmodule R M} `{Rmodule R N} (f:M->N) `{!Rmodule_Morphism f}.
-Definition K : Type := {m: M | f m = mon_unit}.
-Instance: Equiv K := fun k k' => `k = `k'.
-Context (r:R) (k:K).
-Goal f (r <*> `k) = mon_unit.
-rewrite preserves_rmodule_action.
-destruct k; simpl. 
-rewrite e.
-Goal r <*> mon_unit = mon_unit.
-rewrite <- (ginv_l mon_unit) at 1. 
-rewrite rmodule_distr_l.
-apply 
-rewrite (proj2_sig k).
-Program Instance: RalgebraAction R K := fun r k => r <*> ` k.
-Obligation 2.
-apply True.
-Defined.
-Obligation 3.
-destruct k; assumption.
-Qed.
-Obligation 4.
-unfold RalgebraAction_instance_0_obligation_2. auto.
-Defined.
-Obligation 1.
-red.
-intros.
-refine (X <*> `X0).
-
-Typeclasses eauto :=. 
-
+(* TODO: This should be in terms of pointed setoids. *)
+Context `{Monoid M, Monoid N} (f: M→N) `{!Monoid_Morphism f}.
+Definition Kernel := {m: M | f m = mon_unit}.
+Global Instance e: Equiv Kernel := fun k k' => `k = `k'.
+Instance: Equivalence e.
+Global Instance: Setoid Kernel.
+Global Program Instance Kop: SemiGroupOp Kernel := fun k k' => exist _ (`k & `k') _.
 Next Obligation.
- 
+  rewrite preserves_sg_op.
+  destruct k as [k Hk], k' as [k' Hk']; simpl.
+  rewrite Hk, Hk'.
+  apply left_identity.
+Qed.
+Global Instance: Proper (e==>e==>e) sg_op.
+Proof.
+  intros [??][??]?[??][??]?.
+  unfold e; simpl.
+  apply sg_mor; assumption.
+Qed.
+Global Instance: Associative Kop.
+Proof.
+  intros [??][??][??].
+  unfold equiv, e, Kop; simpl.
+  apply (sg_ass _).
+Qed.
+Global Instance: SemiGroup Kernel.
+Global Program Instance: MonoidUnit Kernel := exist _ mon_unit preserves_mon_unit.
+Global Instance: LeftIdentity Kop mon_unit.
+Proof. intros [??]; unfold equiv, e, mon_unit, MonoidUnit_instance_0; simpl; apply left_identity. Qed.
+Global Instance: RightIdentity Kop mon_unit.
+Proof. intros [??]; unfold equiv, e, mon_unit, MonoidUnit_instance_0; simpl; apply right_identity. Qed.
+Global Instance: Monoid Kernel.
+Let  i: Kernel→M := @projT1 _ _.
+Global Instance: Proper (e==>equiv) i.
+Proof. intros [??][??]?; unfold i; simpl; assumption. Qed.
+Global Instance x(*TODO: Name?*): Setoid_Morphism (@projT1 _ _:Kernel->M).
+Global Instance: SemiGroup_Morphism (@projT1 _ _:Kernel->M).
+Proof.
+  constructor; try typeclasses eauto.
+  intros [??][??]; reflexivity.
+Qed.
+Global Instance Monoid_instance_1: Monoid_Morphism (@projT1 _ _:Kernel->M).
+Proof.
+ constructor; try typeclasses eauto; reflexivity.
+Qed.
+Context `{!Commutative sg_op}.
+Global Instance: Commutative (A:=Kernel) sg_op.
+Proof. intros [??][??]; unfold equiv, e; simpl; apply commutativity. Qed.
+End Kernel.
+
+Section Kernel_Group.
+(* TODO: This only needs that M is a monoid. *)
+Context `{Group M, Group N} (f: M→N) `{!Monoid_Morphism f}. 
+Global Program Instance: GroupInv (Kernel f) := fun k => exist _ (-`k) _.
+Next Obligation.
+  destruct k as [k Hk]; simpl.
+  rewrite preserves_inv, Hk; try typeclasses eauto.
+  exact inv_zero.
+Qed.
+Global Instance: Proper (equiv==>equiv) (group_inv (A:=Kernel f)).
+Proof. intros [??][??]?; unfold equiv, e; simpl; apply inv_proper; assumption. Qed.
+(* TODO: Define LeftInverse and RightInverse classes. *)
+Global Instance Kernel_Group: Group `{Kernel f}.
+Proof.
+  constructor; try typeclasses eauto
+  ; intros [??]; unfold equiv, e; simpl; [apply ginv_l | apply ginv_r].
+Qed.
+End Kernel_Group.
+Section Kernel_AbGroup.
+Context `{AbGroup M, AbGroup N} (f: M→N) `{!Monoid_Morphism f}. 
+(* TODO: This only needs a sub semigroup to prove. *)
+Global Instance: AbGroup (Kernel f).
+End Kernel_AbGroup.
+
+Section Kernel_Rmodule.
+Context `{Ring R} `{Rmodule R M, Rmodule R N} (f: M→N) `{!Rmodule_Morphism f}. 
+Global Program Instance rk: RalgebraAction R (Kernel f) := fun r k => exist _ (r<*>` k) _.
+Next Obligation.
+  destruct k as [k Hk]; simpl.
+  rewrite preserves_rmodule_action, Hk.
+  apply preserves_mon_unit.
+Qed.
+Global Instance: !Rmodule R (Kernel f).
+Proof.
+  constructor; try typeclasses eauto; unfold equiv, e, Proper, "==>"; intuition;
+    repeat match goal with 
+      | [ x : Kernel f |- _ ] => destruct x
+    end; simpl.
+  * apply rmodule_unital.
+  * apply rmodule_action_proper; assumption.
+  * apply rmodule_distr_l.
+  * apply rmodule_distr_r.
+  * apply rmodule_assoc.
+Qed.
+
+Global Instance: Rmodule_Morphism (@projT1 _ _:Kernel f→M).
+Proof.
+  constructor; try typeclasses eauto.
+  intros ?[??]; simpl; reflexivity.
+Qed.
+
+End Kernel_Rmodule.
+
 
 Context `{M: nat → Type}.
 Context `{forall n: nat, Rmodule R (e:=e) (M n)}.
